Add absurd and make subtyping lemmas sexier

language_formalisation/type_system/subtyping_lemmas.v
@@ -30,9 +30,8 @@ Lemma sig_subtype_gets_None Σ Σ' op :
   sig_subtype Σ Σ' -> get_op_type Σ' op = None -> get_op_type Σ op = None.
 Proof.
 intros sty gets. induction sty; simpl. reflexivity.
-destruct (op == op0).
-- rewrite e in *. rewrite gets in H. discriminate.
-- apply IHsty. assumption.
+destruct (op == op0); auto.
+rewrite e in *. rewrite gets in H. discriminate.
 Qed.
 
 
@@ -42,13 +41,10 @@ Proof.
 intros.
 induction H.
 + apply SigØsubty.
-+ eapply SigUsubty.
-  - apply IHsig_subtype. assumption.
-  - inv H0. simpl. destruct (op0 == op). 
-    * rewrite e in *. rewrite H1 in H9. discriminate.
-    * exact H1.
-  - assumption.
-  - assumption.
++ eapply SigUsubty; eauto.
+  inv H0. simpl. destruct (op0 == op). 
+  * rewrite e in *. rewrite H1 in H9. discriminate.
+  * exact H1.
 Qed.
 
 
@@ -64,9 +60,7 @@ Lemma eqs_subtype_extend E E' Σ Γ Z T1 T2 :
 Proof.
 intros. induction H.
 apply EqsØsubty.
-eapply EqsUsubty.
-- apply IHeqs_subtype. assumption.
-- simpl. right. assumption.
+eapply EqsUsubty. auto. simpl. right. assumption.
 Qed.
 
 
@@ -75,7 +69,7 @@ Lemma eqs_subtype_contains E E' Γ Z T1 T2 :
 Proof.
 intros sty gets. induction sty; simpl in gets; destruct gets.
 - destruct H0 as [a [b [c ]]]. subst. assumption.
-- apply IHsty. assumption.
+- auto.
 Qed.
 
 
@@ -180,32 +174,28 @@ intros A23; destruct A12; try assumption; inv A23.
 }{
 clear sig_subtype_trans sig_subtype_trans_rev get_op_trans.
 intros A32; destruct A21; try assumption; inv A32. 
-+ apply VsubtyTyΣ.
-  - eapply vsubtype_trans_rev. exact A21_1. assumption.
-  - eapply vsubtype_trans_rev. exact A21_2. assumption.
-+ apply VsubtyTyΠ.
-  - eapply vsubtype_trans_rev. exact A21_1. assumption.
-  - eapply vsubtype_trans_rev. exact A21_2. assumption.
++ apply VsubtyTyΣ; eapply vsubtype_trans_rev; eauto.
++ apply VsubtyTyΠ; eapply vsubtype_trans_rev; eauto.
 + apply VsubtyFun.
-  - eapply vsubtype_trans. exact A21. assumption. 
-  - eapply csubtype_trans_rev. exact H. assumption.
+  - eapply vsubtype_trans; eauto.
+  - eapply csubtype_trans_rev; eauto.
 + apply VsubtyHandler.
-  - eapply csubtype_trans. exact H. assumption. 
-  - eapply csubtype_trans_rev. exact H0. assumption.
+  - eapply csubtype_trans; eauto.
+  - eapply csubtype_trans_rev; eauto.
 }{
 clear vsubtype_trans_rev csubtype_trans csubtype_trans_rev.
 clear sig_subtype_trans_rev get_op_trans.
 intros C23; destruct C12. inv C23. apply Csubty.
-- eapply vsubtype_trans. exact H. assumption.
-- eapply sig_subtype_trans. exact H0. assumption.
-- eapply eqs_subtype_trans. exact H1. assumption.
+- eapply vsubtype_trans; eauto.
+- eapply sig_subtype_trans; eauto.
+- eapply eqs_subtype_trans; eauto.
 }{
 clear vsubtype_trans csubtype_trans csubtype_trans.
 clear sig_subtype_trans get_op_trans.
 intros C32; destruct C21. inv C32. apply Csubty.
-- eapply vsubtype_trans_rev. exact H. assumption.
-- eapply sig_subtype_trans_rev. exact H0. assumption.
-- eapply eqs_subtype_trans. exact H8. assumption.
+- eapply vsubtype_trans_rev; eauto.
+- eapply sig_subtype_trans_rev; eauto.
+- eapply eqs_subtype_trans; eauto.
 }{
 clear csubtype_trans csubtype_trans_rev sig_subtype_trans_rev.
 intros S23. destruct S12.
@@ -213,11 +203,11 @@ apply SigØsubty.
 apply (sig_subtype_gets_Some Σ' Σ3) in H as H'.
 destruct H' as [A'' [B'' [g]]]. eapply SigUsubty.
 2 : exact g. all: try assumption.
-+ eapply sig_subtype_trans. exact S12. assumption.
++ eapply sig_subtype_trans; eauto.
 + clear sig_subtype_trans vsubtype_trans_rev.
-  destruct H2. eapply vsubtype_trans. exact H0. assumption.
+  destruct H2. eapply vsubtype_trans; eauto.
 + clear sig_subtype_trans vsubtype_trans.
-  destruct H2. eapply vsubtype_trans_rev. exact H1. assumption.
+  destruct H2. eapply vsubtype_trans_rev; eauto.
 }{
 clear csubtype_trans csubtype_trans_rev sig_subtype_trans.
 intros S32. destruct S21.
@@ -225,11 +215,9 @@ apply sig_subtype_sigempty in S32. subst. apply SigØsubty.
 induction Σ3.
 apply SigØsubty.
 inv S32. simpl in H8. destruct (o==op).
-+ injection H8. intros. subst. eapply SigUsubty.
-  - apply IHΣ3. assumption.
-  - exact H.
-  - eapply vsubtype_trans_rev. exact H0. assumption.
-  - eapply vsubtype_trans. exact H1. assumption.
++ injection H8. intros. subst. eapply SigUsubty. auto. eauto.
+  - eapply vsubtype_trans_rev; eauto.
+  - eapply vsubtype_trans; eauto.
 + eapply get_op_trans in H8 as gets'.
   2:exact S21. 2:exact H9. 2:exact H10.
   destruct gets' as [A'' [B'' [gets' [styA'']]]]. eapply SigUsubty.
@@ -316,6 +304,7 @@ destruct types. induction H1; apply TypeV; try assumption.
 intros wf ctxsty.
 destruct types. induction H1; apply TypeC; try assumption.
 + apply TypeRet. eapply (ctx_subtype_vtype Γ Γ'); assumption.
++ apply TypeAbsurd. eapply (ctx_subtype_vtype Γ Γ'); assumption.
 + eapply TypeΠMatch.
   - eapply (ctx_subtype_vtype Γ Γ'). exact H1. all: assumption.
   - eapply ctx_subtype_ctype.
@@ -377,6 +366,10 @@ Qed.
 
 (* ========================== Subtype Shapes ========================== *)
 
+Fixpoint subty_shape_empty A : vsubtype A TyØ -> A = TyØ.
+Proof.
+intro sty. inv sty. reflexivity.
+Qed. 
 
 Fixpoint subty_shape_pair A B C : vsubtype C (TyΠ A B) -> 
   exists A' B', C = (TyΠ A' B') /\ vsubtype A' A /\ vsubtype B' B.
@@ -447,6 +440,26 @@ apply (shape_var_full _ _ name num A) in orig as shape.
 Qed.
 
 
+(* Empty *)
+Fixpoint shape_empty_full Γ v A (orig : has_vtype Γ v A) {struct orig} :
+  A = TyØ -> (exists name num, v = Var (name, num)).
+Proof.
+intros samety.
+destruct orig. destruct H1; try discriminate.
++ clear shape_empty_full. exists name. exists num. reflexivity.
++ subst. apply subty_shape_empty in H2. subst.
+  eapply shape_empty_full in H1; auto.
+Qed.
+
+
+Lemma shape_empty Γ v:
+  has_vtype Γ v TyØ -> (exists name num, v = Var (name, num)).
+Proof.
+intro orig.
+apply (shape_empty_full _ _) in orig as shape; auto.
+Qed.
+
+
 (* Pair *)
 Fixpoint shape_pair_full Γ v A B ty (orig : has_vtype Γ v ty) {struct orig} :
   ty = TyΠ A B ->
@@ -457,19 +470,15 @@ intros same.
 destruct orig. destruct H1; try discriminate.
 + clear shape_pair_full. left. exists name. exists num. reflexivity.
 + clear shape_pair_full. right. exists v1. exists v2. 
-  constructor. reflexivity. injection same. intros. subst. 
-  constructor; assumption.
+  constructor. reflexivity. injection same. intros. subst. auto. 
 + rewrite same in H2. apply subty_shape_pair in H2. 
   destruct H2 as [A'' [B'' [pity]]]. subst. 
   apply (shape_pair_full _ _ A'' B'') in H1. clear shape_pair_full. 
-  2: reflexivity. destruct H1.
-  - left. assumption.
-  - right. destruct H1 as [v1 [v2]]. exists v1. exists v2.
-    constructor. destruct H1. assumption.
-    constructor; destruct H1; destruct H3; destruct H2;
-    apply TypeV; inv H0; try assumption. 
-    * eapply TypeVSubtype. exact H3. assumption.
-    * eapply TypeVSubtype. exact H4. assumption.
+  2: reflexivity. destruct H1. auto.
+  right. destruct H1 as [v1 [v2]]. exists v1. exists v2.
+  constructor. destruct H1. assumption.
+  constructor; destruct H1; destruct H3; destruct H2;
+  apply TypeV; inv H0; try assumption; eapply TypeVSubtype; eauto.
 Qed.
 
 
@@ -495,22 +504,19 @@ Proof.
 intros same.
 destruct orig. destruct H1; try discriminate.
 + clear shape_sum_full. left. exists name. exists num. reflexivity.
-+ clear shape_sum_full. right. left. exists v. constructor. reflexivity.
-  inv same. assumption.
-+ clear shape_sum_full. right. right. exists v. constructor. reflexivity.
-  inv same. assumption.
++ clear shape_sum_full. right. left. exists v. inv same. auto.
++ clear shape_sum_full. right. right. exists v. inv same. auto.
 + rewrite same in H2. apply subty_shape_sum in H2. 
   destruct H2 as [A'' [B'' [sigty]]]. subst. 
   apply (shape_sum_full _ _ A'' B'') in H1. clear shape_sum_full. 
-  2: reflexivity. destruct H1.
-  - left. assumption.
-  - right. destruct H1.
-    * left. destruct H1. exists x. destruct H1. constructor. assumption.
-      apply TypeV. assumption. inv H0. assumption. eapply TypeVSubtype.
-      exact H3. destruct H2. assumption.
-    * right. destruct H1. exists x. destruct H1. constructor. assumption.
-      apply TypeV. assumption. inv H0. assumption. eapply TypeVSubtype.
-      exact H3. destruct H2. assumption.
+  2: reflexivity. destruct H1. auto.
+  right. destruct H1.
+  * left. destruct H1. exists x. destruct H1. constructor. assumption.
+    apply TypeV. assumption. inv H0. assumption. destruct H2.
+    eapply TypeVSubtype; eauto.
+  * right. destruct H1. exists x. destruct H1. constructor. assumption.
+    apply TypeV. assumption. inv H0. assumption. destruct H2.
+    eapply TypeVSubtype; eauto.
 Qed.
 
 
@@ -521,9 +527,7 @@ intro orig.
 apply (shape_sum_full _ _ A B) in orig as shape. 2: reflexivity.
 destruct shape.
 + destruct H as [name [num]]. discriminate.
-+ destruct H; destruct H; destruct H.
-  - inv H. assumption.
-  - discriminate.
++ destruct H; destruct H; destruct H; inv H. auto.
 Qed.
 
 
@@ -534,9 +538,7 @@ intro orig.
 apply (shape_sum_full _ _ A B) in orig as shape. 2: reflexivity.
 destruct shape.
 + destruct H as [name [num]]. discriminate.
-+ destruct H; destruct H; destruct H.
-  - discriminate.
-  - inv H. assumption.
++ destruct H; destruct H; destruct H; inv H. auto.
 Qed.
 
 
@@ -554,17 +556,16 @@ destruct orig. destruct H1; try discriminate.
 + rewrite same in H2. apply subty_shape_fun in H2. 
   destruct H2 as [A'' [C'' [funty]]]. subst. 
   apply (shape_fun_full _ _ A'' C'') in H1. clear shape_fun_full. 
-  2: reflexivity. destruct H1.
-  - left. assumption.
-  - right. destruct H1. destruct H1 as [c']. exists x. exists c'.
-    destruct H1. constructor. assumption.
-    apply TypeC; inv H0.
-    * apply WfCtxU; assumption.
-    * assumption.
-    * destruct H2. eapply TypeCSubtype. 2: exact H1.
-      eapply ctx_subtype_ctype. exact H3.
-      apply WfCtxU; assumption.
-      apply CtxUsubty. apply ctx_subty_refl. assumption. assumption.
+  2: reflexivity. destruct H1. auto.
+  right. destruct H1. destruct H1 as [c']. exists x. exists c'.
+  destruct H1. constructor. assumption.
+  apply TypeC; inv H0.
+  * apply WfCtxU; assumption.
+  * assumption.
+  * destruct H2. eapply TypeCSubtype. 2: exact H1.
+    eapply ctx_subtype_ctype. exact H3.
+    apply WfCtxU; assumption.
+    apply CtxUsubty. apply ctx_subty_refl. assumption. assumption.
 Qed.
 
 Lemma shape_fun Γ x c A C :
@@ -594,20 +595,18 @@ destruct orig. destruct H1; try discriminate.
   destruct H2 as [C' [D' [hty]]]. destruct H2. subst.
   destruct C' as [A' Σ' E'].
   apply (shape_handler_full _ _ A' Σ' E' D') in H1.
-  clear shape_handler_full. 2: reflexivity. destruct H1.
-  left. assumption.
+  clear shape_handler_full. 2: reflexivity. destruct H1. auto.
   right. destruct H1 as [x [cr [h [same]]]]. exists x. exists cr. exists h.
   destruct H1. constructor. assumption. constructor.
   - apply TypeC; inv H0.
-    * apply WfCtxU. assumption. inv H7. assumption.
+    * inv H7. apply WfCtxU; auto.
     * assumption.
     * eapply TypeCSubtype. 2: exact H3.
       eapply ctx_subtype_ctype. exact H1.
-      apply WfCtxU. assumption. inv H7. assumption.
-      apply CtxUsubty. apply ctx_subty_refl. assumption. 
-      inv H2. assumption.
+      inv H7. apply WfCtxU; auto.
+      inv H2. apply CtxUsubty. apply ctx_subty_refl. all: assumption. 
   - apply TypeH; inv H0; try assumption. inv H7. assumption.
-    eapply TypeHSubtype. exact H4. inv H2. assumption. assumption. 
+    inv H2. eapply TypeHSubtype; eauto.
 Qed.
 
 Lemma shape_handler Γ x c_r h A Σ E D:
@@ -621,7 +620,59 @@ destruct shape.
 + do 3 (destruct H). inv H. inv H0. assumption.
 Qed.
 
+(* ========================= Handler Cases Shapes ========================= *)
+
+Fixpoint shape_casesempty_full Γ h Σ D
+  (orig : has_htype Γ h Σ D) {struct orig} :
+  h = CasesØ -> Σ = SigØ.
+Proof.
+intros same.
+destruct orig. destruct H2; try discriminate.
++ reflexivity.
++ apply shape_casesempty_full in H2. 2: assumption.
+  subst. apply sig_subtype_sigempty. assumption.
+Qed.
+
 (* ========================== Computation Shapes ========================== *)
+
+
+(* Return *)
+Fixpoint shape_ret_full Γ c C v A Σ E
+  (orig : has_ctype Γ c C) {struct orig} :
+  c = (Ret v) -> C = (CTy A Σ E) -> has_vtype Γ v A.
+Proof.  
+intros same samety. destruct orig. destruct H1; try discriminate.
++ clear shape_ret_full. inv same. inv samety. assumption.
++ destruct C as (A', Σ', E').
+  apply (shape_ret_full _ _ (CTy A' Σ' E') v A' Σ' E') in H1;
+  clear shape_ret_full; auto. subst.
+  inv H0. apply TypeV; auto.
+  inv H2. eapply TypeVSubtype; eauto.
+Qed.
+
+
+Fixpoint shape_ret Γ v A Σ E :
+  has_ctype Γ (Ret v) (CTy A Σ E) -> has_vtype Γ v A.
+Proof.  
+intro orig. eapply (shape_ret_full _ _ _ v A Σ E) in orig; auto.
+Qed.
+
+
+(* Return *)
+Fixpoint shape_absurd_full Γ c C v (orig : has_ctype Γ c C) {struct orig} :
+  c = (Absurd v) -> has_vtype Γ v TyØ.
+Proof.  
+intros same. destruct orig. destruct H1; try discriminate; inv same.
++ assumption.
++ apply (shape_absurd_full _ _ _ v) in H1; auto.
+Qed.
+
+
+Fixpoint shape_absurd Γ v C :
+  has_ctype Γ (Absurd v) C -> has_vtype Γ v TyØ.
+Proof.  
+intro orig. eapply (shape_absurd_full _ _ _ v) in orig; auto.
+Qed.
 
 
 (* ΠMatch *)
@@ -632,14 +683,14 @@ Fixpoint shape_prodmatch_full Γ c v x y c' C
 Proof.  
 intros same. destruct orig. destruct H1; try discriminate.
 + clear shape_prodmatch_full. 
-  inv same. exists A. exists B. constructor; assumption.
+  inv same. exists A. exists B. auto.
 + apply (shape_prodmatch_full _ _ v x y c') in H1; clear shape_prodmatch_full. 
   2: assumption. destruct H1 as [A' [B' [vty]]].
   exists A'. exists B'. constructor. assumption.
   apply TypeC.
   - inv H1. assumption.
   - assumption.
-  - eapply TypeCSubtype. exact H1. assumption.
+  - eapply TypeCSubtype; eauto.
 Qed.
 
 
@@ -647,8 +698,7 @@ Fixpoint shape_prodmatch Γ v x y c C :
   has_ctype Γ (ΠMatch v (x, y) c) C ->
   (exists A B, has_vtype Γ v (TyΠ A B) /\  has_ctype (CtxU (CtxU Γ A) B) c C).
 Proof.
-intro orig. apply (shape_prodmatch_full _ _ v x y c) in orig.
-2: reflexivity. assumption.
+intro orig. apply (shape_prodmatch_full _ _ v x y c) in orig; auto.
 Qed.
 
 
@@ -660,18 +710,16 @@ Fixpoint shape_summatch_full Γ c v xl cl xr cr C
     has_ctype (CtxU Γ A) cl C /\ has_ctype (CtxU Γ B) cr C).
 Proof.  
 intros same. destruct orig. destruct H1; try discriminate.
-+ clear shape_summatch_full. 
-  inv same. exists A. exists B. constructor. assumption.
-  constructor ; assumption.
++ clear shape_summatch_full. inv same. exists A. exists B. auto.
 + apply (shape_summatch_full _ _ v xl cl xr cr) in H1;
   clear shape_summatch_full. 2: assumption.
   destruct H1 as [A' [B' [vty]]].
   exists A'. exists B'. constructor. assumption.
   inv H1. constructor; apply TypeC; auto.
   - inv H3. assumption.
-  - eapply TypeCSubtype. exact H3. assumption.
+  - eapply TypeCSubtype; eauto.
   - inv H4. assumption.
-  - eapply TypeCSubtype. exact H4. assumption.
+  - eapply TypeCSubtype; eauto.
 Qed.
 
 
@@ -680,10 +728,8 @@ Fixpoint shape_summatch Γ v xl cl xr cr C :
   (exists A B, has_vtype Γ v (TyΣ A B) /\
     has_ctype (CtxU Γ A) cl C /\ has_ctype (CtxU Γ B) cr C).
 Proof.
-intro orig. apply (shape_summatch_full _ _ v xl cl xr cr) in orig.
-2: reflexivity. assumption.
+intro orig. apply (shape_summatch_full _ _ v xl cl xr cr) in orig; auto.
 Qed.
-
 
 (* App *)
 Fixpoint shape_app_full Γ c v1 v2 C (orig : has_ctype Γ c C) {struct orig} :
@@ -691,7 +737,7 @@ Fixpoint shape_app_full Γ c v1 v2 C (orig : has_ctype Γ c C) {struct orig} :
   (exists A, has_vtype Γ v1 (TyFun A C) /\ has_vtype Γ v2 A).
 Proof.  
 intros same. destruct orig. destruct H1; try discriminate.
-+ clear shape_app_full. inv same. exists A. constructor; assumption.
++ clear shape_app_full. inv same. exists A. auto.
 + apply (shape_app_full _ _ v1 v2) in H1;
   clear shape_app_full. 2: assumption.
   destruct H1 as [A' [fty]].
@@ -719,24 +765,21 @@ Fixpoint shape_handle_full Γ c v c' C (orig : has_ctype Γ c C) {struct orig} :
   (exists C', has_vtype Γ v (TyHandler C' C) /\ has_ctype Γ c' C').
 Proof.  
 intros same. destruct orig. destruct H1; try discriminate.
-+ clear shape_handle_full. 
-  inv same. exists C. constructor; assumption.
++ clear shape_handle_full. inv same. exists C. auto.
 + apply (shape_handle_full _ _ v c') in H1;
   clear shape_handle_full. 2: assumption.
   destruct H1 as [D [vty]].
-  exists D. constructor. 2: assumption.
-  apply TypeV. assumption. apply WfHandler. inv H1. assumption. assumption.
+  exists D. constructor. 2: assumption. inv H1.
+  apply TypeV. assumption. apply WfHandler; auto.
   eapply TypeVSubtype. exact vty.
-  apply VsubtyHandler. apply csubtype_refl. inv H1. assumption. assumption.
+  apply VsubtyHandler. apply csubtype_refl. all: assumption.
 Qed.
-
 
 Fixpoint shape_handle Γ v c D :
   has_ctype Γ (Handle v c) D ->
   (exists C, has_vtype Γ v (TyHandler C D) /\ has_ctype Γ c C).
 Proof.
-intro orig. eapply (shape_handle_full _ _ v c D) in orig.
-2: reflexivity. assumption.
+intro orig. eapply (shape_handle_full _ _ v c D) in orig; auto.
 Qed.
 
 
@@ -748,8 +791,7 @@ Fixpoint shape_letrec_full Γ c f x c1 c2 D
   has_ctype (CtxU Γ (TyFun A C)) c2 D).
 Proof.  
 intros same. destruct orig. destruct H1; try discriminate.
-+ clear shape_letrec_full. 
-  inv same. exists A. exists C. constructor; assumption.
++ clear shape_letrec_full. inv same. exists A. exists C. auto.
 + apply (shape_letrec_full _ _ f x c1 c2) in H1;
   clear shape_letrec_full. 2: assumption.
   destruct H1 as [A' [C'' [cty]]].
@@ -764,8 +806,7 @@ Fixpoint shape_letrec Γ f x c1 c2 D :
   (exists A C, has_ctype (CtxU (CtxU Γ A) (TyFun A C)) c1 C /\ 
     has_ctype (CtxU Γ (TyFun A C)) c2 D).
 Proof.
-intro orig. eapply (shape_letrec_full _ _ f x c1 c2 D) in orig.
-2: reflexivity. assumption.
+intro orig. eapply (shape_letrec_full _ _ f x c1 c2 D) in orig; auto.
 Qed.
 
 
@@ -776,19 +817,17 @@ Fixpoint shape_dobind_full Γ c C x c1 c2 A Σ E
   (exists A', has_ctype Γ c1 (CTy A' Σ E) /\ has_ctype (CtxU Γ A') c2 C).
 Proof.  
 intros same samety. destruct orig. destruct H1; try discriminate; inv same.
-+ inv samety. clear shape_dobind_full. 
-  exists A0. constructor; assumption.
++ inv samety. clear shape_dobind_full. exists A0. auto.
 + destruct C as (A', Σ', E').
   apply (shape_dobind_full _ _ (CTy A' Σ' E') x c1 c2 A' Σ' E') in H1;
-  clear shape_dobind_full. 2: reflexivity. 2: reflexivity.
-  destruct H1 as [A'' [cty]].
+  clear shape_dobind_full; auto. destruct H1 as [A'' [cty]].
   exists A''. constructor.
   - apply TypeC. assumption. inv cty. inv H0. inv H4.
     apply WfCty; assumption. eapply TypeCSubtype. exact cty.
      inv H2. inv cty. inv H3. 
     apply Csubty. apply vsubtype_refl. all: assumption.
   - apply TypeC. inv H1. assumption. assumption.
-    eapply TypeCSubtype. exact H1. assumption.
+    eapply TypeCSubtype; eauto.
 Qed.
 
 
@@ -797,32 +836,9 @@ Fixpoint shape_dobind Γ x c1 c2 A Σ E :
   (exists A', has_ctype Γ c1 (CTy A' Σ E) /\ 
     has_ctype (CtxU Γ A') c2 (CTy A Σ E)).
 Proof.  
-intro orig. eapply (shape_dobind_full _ _ _ x c1 c2 A Σ E) in orig.
-2: reflexivity. assumption. reflexivity.
+intro orig. eapply (shape_dobind_full _ _ _ x c1 c2 A Σ E) in orig; auto.
 Qed.
 
-
-(* Return *)
-Fixpoint shape_ret_full Γ c C v A Σ E
-  (orig : has_ctype Γ c C) {struct orig} :
-  c = (Ret v) -> C = (CTy A Σ E) -> has_vtype Γ v A.
-Proof.  
-intros same samety. destruct orig. destruct H1; try discriminate; inv same.
-+ inv samety. assumption.
-+ destruct C as (A', Σ', E').
-  apply (shape_ret_full _ _ (CTy A' Σ' E') v A' Σ' E') in H1;
-  clear shape_ret_full. 2: reflexivity. 2: reflexivity.
-  - apply TypeV. assumption. inv H0. assumption.
-    eapply TypeVSubtype. exact H1. inv H2. assumption.
-Qed.
-
-
-Fixpoint shape_ret Γ v A Σ E :
-  has_ctype Γ (Ret v) (CTy A Σ E) -> has_vtype Γ v A.
-Proof.  
-intro orig. eapply (shape_ret_full _ _ _ v A Σ E) in orig.
-2: reflexivity. assumption. reflexivity.
-Qed.
 
 (* Op *)
 Fixpoint shape_op_full Γ c C op v y c' A Σ E
@@ -832,9 +848,7 @@ Fixpoint shape_op_full Γ c C op v y c' A Σ E
   has_vtype Γ v Aop /\  has_ctype (CtxU Γ Bop) c' C).
 Proof.  
 intros same samety. destruct orig. destruct H1; try discriminate; inv same.
-+ inv samety. clear shape_op_full. 
-  exists A_op. exists B_op.
-  constructor. assumption. constructor; assumption.
++ inv samety. clear shape_op_full. exists A_op. exists B_op. auto.
 + destruct C as (A', Σ', E').
   apply (shape_op_full _ _ (CTy A' Σ' E') op v y c' A' Σ' E') in H1;
   clear shape_op_full. 2: reflexivity. 2: reflexivity.
@@ -850,8 +864,8 @@ intros same samety. destruct orig. destruct H1; try discriminate; inv same.
     * apply TypeC. inv H1. assumption. assumption.
       eapply TypeCSubtype. exact H1. apply Csubty; assumption.
     * apply WfCtxU. assumption. apply get_op_type_wf in g'. destruct g'.
-      assumption. inv H0. assumption.
-    * apply CtxUsubty. apply ctx_subty_refl. assumption. assumption.
+      all: inv H0; assumption.
+    * apply CtxUsubty. apply ctx_subty_refl. all: assumption.
 Qed.
 
 
@@ -860,6 +874,5 @@ Fixpoint shape_op Γ op v y c A Σ E :
   (exists Aop Bop, get_op_type Σ op = Some (Aop, Bop) /\
     has_vtype Γ v Aop /\  has_ctype (CtxU Γ Bop) c (CTy A Σ E)).
 Proof.  
-intro orig. eapply (shape_op_full _ _ _ op v y c A Σ E) in orig.
-2: reflexivity. assumption. reflexivity.
+intro orig. eapply (shape_op_full _ _ _ op v y c A Σ E) in orig; auto.
 Qed.
